src/crypto/aes/aes-x64/gcm_helpers.i.dfy
@@ -28,30 +28,182 @@ lemma lemma_BitwiseAdd32()
     reveal_BitwiseAdd32();
 }
 
-/*
-// It's not clear to me what is the best way to allow proof.
-// 0b00010000 
-function uint8Tobv8(b : uint8) : bv8 { b as bv8 }
-
-// Whoa, where are bit vectors specified?
-predicate isbv8eq0(b : bv8) {
-  b[0] == 0
+// Testing bits, not known if it proves well yet.
+predicate BitTest8(x : bv8, amount : int)
+  requires 0 <= amount < 8;
+{
+   ((x >> amount) & 0x1) == 1
 }
 
+predicate BitTest16(x : bv16, amount : int)
+  requires 0 <= amount < 16;
+{
+   ((x >> amount) & 0x1) == 1
+}
+
+predicate BitTest32(x : bv32, amount : int)
+  requires 0 <= amount < 32;
+{
+   ((x >> amount) & 0x1) == 1
+}
+
+predicate BitTest64(x : bv64, amount : int)
+  requires 0 <= amount < 64;
+{
+   ((x >> amount) & 0x1) == 1
+}
+
+predicate BitTest128(x : bv128, amount : int)
+  requires 0 <= amount < 128;
+{
+   ((x >> amount) & 0x1) == 1
+}
+
+/* 
+// Sanity checks.
+
+// Does z3 shift off to the left correctly. Yes.
+lemma is_shift_off_correct_64()
+ ensures (0x8000_0000_0000_0000 as bv64) << 1 == 0;
+ ensures (0x9000_0000_0000_0000 as bv64) << 1 != 0;
+{}
+
+lemma is_shift_on_zero_64()
+ ensures forall b : bv64 :: (b << 1) & (0x1 as bv64) == 0;
+ ensures forall b : bv64 :: (b << 1) % 2 == 0;
+ ensures forall b : bv64 :: (b << 2) % (0x1 << 2) == 0;
+ ensures forall b : bv64 :: (b << 64) == 0;
+{}
+
+*/
+
+/*
+// Proves in 45 s.
+lemma lemma_ShiftsAdd(x: bv8, a: nat, b: nat)
+  requires 0 <= a + b < 8
+  ensures x << (a + b) == (x << a) << b;
+{
+  forall i : nat | a + i < 8
+   ensures x << (a + i) == (x << a) << i
+   {
+    forall j : nat | j + i < 8
+     ensures x << (j + i) == (x << j) << i
+     {
+     }
+   }
+}
+*/
+
+/*
+// Proves in 1:27 s.
+lemma {:timeLimitMultiplier 3} lemma_ShiftsAdd(x: bv16, a: nat, b: nat)
+  requires 0 <= a + b < 16
+  ensures x << (a + b) == (x << a) << b;
+{
+  forall i : nat | a + i < 16
+   ensures x << (a + i) == (x << a) << i
+   {
+    forall j : nat | j + i < 16
+     ensures x << (j + i) == (x << j) << i
+     {
+     }
+   }
+}
+*/
+/*
+lemma {:timeLimitMultiplier 6} lemma_ShiftsAdd(x: bv32, a: nat, b: nat)
+  requires 0 <= a + b < 32;
+  ensures x << (a + b) == (x << a) << b;
+{
+  forall i : nat | a + i < 32
+   ensures x << (a + i) == (x << a) << i
+   {
+    forall j : nat | j + i < 32
+     ensures x << (j + i) == (x << j) << i
+     {
+     }
+   }
+}
+*/
+
+/*
+lemma lemma_left_shift_zero()
+ ensures forall b : bv64 :: b == b << 0;
+{}
+
+lemma left_shift_to_math_fix(b : bv64, i : nat)
+  requires i <= 64;
+  ensures b << i == (((b as int) * power(2,i)) % 0x1_0000_0000_0000_0000) as bv64;
+{
+  if (i == 0) {
+    lemma_left_shift_zero();
+    assert b << i == b;
+    assert power(2,0) == 1;
+    assert (b as int) * 1 == b as int;
+    assert (b as int) < 0x1_0000_0000_0000_0000;
+    assert (b as int) % 0x1_0000_0000_0000_0000 == (b as int);
+  }
+  else { 
+    left_shift_to_math_fix(b, i - 1);
+  }
+}
+
+lemma left_shift_cummulative_fix(b : bv64, i : nat, j : nat)
+ requires i + j <= 64;
+ ensures b << (i + j) == (b << i) << j;
+{
+  if (i == 0) { } 
+  else {
+   left_shift_cummulative_fix(b, i - 1, j);
+ }
+}
+*/
+
+/*
+lemma left_shift_cummulative()
+ ensures forall b : bv64 :: forall i : nat :: forall j : nat :: 
+ i + j <= 64 ==> b << (i + j) == (b << i) << j;
+{ forall k : 
+
+}
+*/
+
+/*
 method CL_MUL_SHIFT(a : bv64, b : bv64) returns (r : bv128)
 {
-   var a' := a;
-   var b' := b;
-   r := 0;
-    while b' != 0
+  var a' := a;
+  var b' := b;
+  var i := 0;
+  r := 0;
+  assume b == 0 || exists i : nat :: i <= 8 ==> b << i == 0;
+  while b' != 0
+   decreases 64 - i;
   {
      if ((a' & 1) != 0) {
-          r := r ^ b';
+      r := r ^ (b' as bv128);
      }
     a' := a' >> 1;
     b' := b' << 1;
+    i := i + 1;
+    assume b' == b << i;
  }
 }
+*/
+
+/*
+function CL_MUL_SHIFT'(a : bv64, b : bv64, r : bv128) : bv128
+{
+ if b != 0 then
+   if ((a & 1) != 0) then
+     CL_MUL_SHIFT'(a >> 1, b << 1, r ^ (b as bv128))
+   else 
+     CL_MUL_SHIFT'(a >> 1, b << 1, r)
+ else 
+  r
+}
+*/
+
+/*
 
 method CL_MUL(src1 : bv128, src2 : bv128, imm8 : bv8) returns (dest : bv128) 
 {
@@ -59,18 +211,17 @@ method CL_MUL(src1 : bv128, src2 : bv128, imm8 : bv8) returns (dest : bv128)
   var temp2 : bv128;
 
   if (imm8[0] == 0) {
-    temp1 := src1[63:0];
+    temp1 := src1 % 0x1_0000_0000_0000_0000;
   } else {
-    temp1 := src1[127:64];
+    temp1 := src1 / 0x1_0000_0000_0000_0000;
   }
 
   if (imm8[4] == 0) {
-    temp2 := src2[63:0];
+    temp2 := src2 % 0x1_0000_0000_0000_0000;
   } else {
-    temp2 := src2[127:64];
+    temp2 := src2 / 0x1_0000_0000_0000_0000;
   }
 
-  var dest : bv128;
   var i := 0;
   var tempb : bv128;
   while (i <= 63) {
@@ -97,7 +248,6 @@ method CL_MUL(src1 : bv128, src2 : bv128, imm8 : bv8) returns (dest : bv128)
   } 
   dest[127] := 0;
 }
-
 */
 
 }
